`AddSummary.lean`: add `SIGNEXTEND` opcode summary

EvmEquivalence/Summaries/AddSummary.lean
@@ -16,6 +16,7 @@ inductive arith_op where
 | sdiv
 | mod
 | smod
+| signextend
 deriving BEq, DecidableEq
 
 section
@@ -40,6 +41,7 @@ abbrev divEVM := @Operation.DIV .EVM
 abbrev sdivEVM := @Operation.SDIV .EVM
 abbrev modEVM := @Operation.MOD .EVM
 abbrev smodEVM := @Operation.SMOD .EVM
+abbrev signextendEVM := @Operation.SIGNEXTEND .EVM
 
 abbrev add_instr : Option (Operation .EVM × Option (UInt256 × Nat)) := some ⟨addEVM, none⟩
 abbrev sub_instr : Option (Operation .EVM × Option (UInt256 × Nat)) := some ⟨subEVM, none⟩
@@ -47,6 +49,7 @@ abbrev div_instr : Option (Operation .EVM × Option (UInt256 × Nat)) := some �
 abbrev sdiv_instr : Option (Operation .EVM × Option (UInt256 × Nat)) := some ⟨sdivEVM, none⟩
 abbrev mod_instr : Option (Operation .EVM × Option (UInt256 × Nat)) := some ⟨modEVM, none⟩
 abbrev smod_instr : Option (Operation .EVM × Option (UInt256 × Nat)) := some ⟨smodEVM, none⟩
+abbrev signextend_instr : Option (Operation .EVM × Option (UInt256 × Nat)) := some ⟨signextendEVM, none⟩
 
 @[simp]
 def arith_op.get : (Option (Operation .EVM × Option (UInt256 × Nat))) :=
@@ -57,6 +60,7 @@ def arith_op.get : (Option (Operation .EVM × Option (UInt256 × Nat))) :=
   | .sdiv => sdiv_instr
   | .mod  => mod_instr
   | .smod => smod_instr
+  | .signextend => signextend_instr
 
 --@[simp]
 def arith_op.t : Operation .EVM :=
@@ -67,6 +71,7 @@ def arith_op.t : Operation .EVM :=
   | .sdiv => (sdiv_instr.get rfl).1
   | .mod => (mod_instr.get rfl).1
   | .smod => (smod_instr.get rfl).1
+  | .signextend => (signextend_instr.get rfl).1
 
 def EVM.step_arith : Transformer := EVM.step gas gasCost op.get
 
@@ -81,6 +86,7 @@ def arith_op.do :=
   | .sdiv => word₁.sdiv word₂
   | .mod  => word₁.mod word₂
   | .smod  => word₁.smod word₂
+  | .signextend => word₁.signextend word₂
 
 theorem EvmYul.step_sub_summary (symState : EVM.State):
   EvmYul.step_arith op {symState with
@@ -204,6 +210,7 @@ def arith_op.to_bin : ByteArray :=
   | .sdiv => ⟨#[0x5]⟩
   | .mod  => ⟨#[0x6]⟩
   | .smod => ⟨#[0x7]⟩
+  | .signextend => ⟨#[0xB]⟩
 
 @[simp]
 theorem decode_singleton_add :
@@ -223,6 +230,9 @@ theorem decode_singleton_mod :
 @[simp]
 theorem decode_singleton_smod :
   decode ⟨#[0x7]⟩ (.ofNat 0) = some ⟨smodEVM, none⟩ := rfl
+@[simp]
+theorem decode_singleton_signextend :
+  decode ⟨#[0xB]⟩ (.ofNat 0) = some ⟨signextendEVM, none⟩ := rfl
 
 @[simp]
 theorem decode_singleton_arith :
